sim: Try to shrink commit/reset functions
- Don't commit/reset state for registers that are only read
- Don't commit/reset rwsets for registers that are only read at port 0

This yields a 5% or so speedup on the processor in GCC, mostly in
Decode (previously, that rule's reset and commit functions would copy the
register file, not just the scoreboard).  It doesn't seem to
affect Clang much.

ocaml/backends/cpp.ml
@@ -2,6 +2,8 @@
 open Common
 module Extr = Cuttlebone.Extr
 
+let debug = false
+
 (* #line pragmas make the C++ code harder to read, and they cover too-large a
    scope (in particular, the last #line pragma in a program overrides positions
    for all subsequent code, while we'd want to use the C++ positions for these
@@ -19,7 +21,7 @@ let use_offsets_in_dynamic_log = false
 type ('pos_t, 'var_t, 'fn_name_t, 'rule_name_t, 'reg_t, 'ext_fn_t) cpp_rule_t = {
     rl_external: bool;
     rl_name: 'rule_name_t;
-    rl_footprint: 'reg_t array;
+    rl_reg_histories: 'reg_t -> Extr.register_history;
     rl_body: (('pos_t, 'reg_t) Extr.register_annotation,
               'var_t, 'fn_name_t, 'reg_t, 'ext_fn_t) Extr.rule;
   }
@@ -670,15 +672,16 @@ let compile (type pos_t var_t fn_name_t rule_name_t reg_t ext_fn_t)
       nl ());
     p "#include \"%s\"" cuttlesim_hpp_fname in
 
-  let reg_sig_w_kind r =
-    (hpp.cpp_register_kinds r, hpp.cpp_register_sigs r) in
+  let iter_registers f regs =
+    let sigs = Array.map hpp.cpp_register_sigs regs in
+    Array.iter f sigs in
 
-  let iter_registers_with_kinds f regs =
-    Array.iter (fun r -> f (reg_sig_w_kind r)) regs in
-
-  let iter_all_registers =
+  let iter_all_registers = (* Note the late binding of ‘f’ *)
     let sigs = Array.map hpp.cpp_register_sigs hpp.cpp_registers in
     fun f -> Array.iter f sigs in
+
+  let reg_sig_w_kind r =
+    (hpp.cpp_register_kinds r, hpp.cpp_register_sigs r) in
 
   let iter_all_registers_with_kind =
     let sigs = Array.map reg_sig_w_kind hpp.cpp_registers in
@@ -827,11 +830,45 @@ let compile (type pos_t var_t fn_name_t rule_name_t reg_t ext_fn_t)
     let p_rule (rule: (pos_t, var_t, fn_name_t, rule_name_t, reg_t, ext_fn_t) cpp_rule_t) =
       gensym_reset ();
 
-      let footprint_sz =
-        Array.length rule.rl_footprint in
+      let filter_registers_by_history cond =
+        List.filter (fun reg -> cond reg (rule.rl_reg_histories reg))
+          (Array.to_list hpp.cpp_registers)
+        |> Array.of_list in
 
-      let large_footprint =
-        5 * footprint_sz > 4 * Array.length hpp.cpp_registers in
+      let rwset_footprint =
+        (* No need to save or reset a register's read-write set if it's only
+           read at port 0, or if it's a value (i.e. a register for which reads
+           and writes cannot fail in any rule, in which case we don't generate a
+           read-write set at all). *)
+        filter_registers_by_history (fun reg { hr1; hw0; hw1; _ } ->
+            hpp.cpp_register_kinds reg <> Value &&
+            Extr.(hr1 <> TFalse || hw0 <> TFalse || hw1 <> TFalse)) in
+
+      let rwdata_footprint =
+        (* No need to save or reset a register's data if it's only read *)
+        filter_registers_by_history (fun _reg { hw0; hw1; _ } ->
+            Extr.(hw0 <> TFalse || hw1 <> TFalse)) in
+
+      if debug then (
+        let debug_footprint name fp =
+          Printf.printf "Footprints for %s in %s:\n"
+            name (hpp.cpp_rule_names rule.rl_name);
+          Array.iter (fun r ->
+              let nm = (hpp.cpp_register_sigs r).reg_name in
+              let rfp = rule.rl_reg_histories r in
+              let pr = function
+                | Extr.TTrue -> "true"
+                | Extr.TFalse -> "false"
+                | Extr.TUnknown -> "?" in
+              Printf.printf "  %s: {r0=%s; r1=%s; w0=%s; w1=%s; cf=%s}\n" nm
+                (pr rfp.hr0) (pr rfp.hr1) (pr rfp.hw0) (pr rfp.hw1) (pr rfp.hcf))
+            fp in
+
+        debug_footprint "rwset" rwset_footprint;
+        debug_footprint "rwdata" rwdata_footprint);
+
+      let large_footprint footprint = (* FIXME should be tweaked based on the speed of memset *)
+        5 * Array.length footprint > 4 * Array.length hpp.cpp_registers in
 
       let rule_max_log_size =
         Extr.rule_max_log_size rule.rl_body in
@@ -840,7 +877,8 @@ let compile (type pos_t var_t fn_name_t rule_name_t reg_t ext_fn_t)
         (* LATER: Refine this criterion based on rule_max_log_size; at the moment
            this measure isn't precise enough to be truly useful, because it
            overestimates log sizes in imperative switches. *)
-        use_dynamic_logs && footprint_sz > 10 in
+        use_dynamic_logs && (Array.length rwdata_footprint > 10 ||
+                              Array.length rwset_footprint > 10) in
 
       let dl_suffix =
         if use_dynamic_log
@@ -855,24 +893,26 @@ let compile (type pos_t var_t fn_name_t rule_name_t reg_t ext_fn_t)
           sprintf "READ%d%s" pt (rw_suffix reg) in
       let write reg pt = sprintf "WRITE%d%s" pt (rw_suffix reg) in
 
-      let p_copy exclude_values field src dst =
+      let p_copy field src dst footprint =
         let src = sprintf "%s.%s" src field in
         let dst = sprintf "%s.%s" dst field in
-        iter_registers_with_kinds (function
-            | (Value, _) when exclude_values -> ()
-            | (_, { reg_name; _ }) ->
-               p "%s.%s = %s.%s;" dst reg_name src reg_name)
-          rule.rl_footprint in
+        if large_footprint footprint then
+          p "%s = %s;" dst src
+        else
+          iter_registers (fun { reg_name; _ } ->
+              p "%s.%s = %s.%s;" dst reg_name src reg_name)
+            footprint in
 
-      let p_reset () =
-        if large_footprint then p "log = Log;"
-        else (p_copy false "state" "Log" "log";
-              p_copy true "rwset" "Log" "log") in
+      let p_commit_reset src dst =
+        if large_footprint rwdata_footprint &&
+             large_footprint rwset_footprint then
+          p "%s = %s;" dst src
+        else (
+          p_copy "state" src dst rwdata_footprint;
+          p_copy "rwset" src dst rwset_footprint) in
 
-      let p_commit () =
-        if large_footprint then p "Log = log;"
-        else (p_copy false "state" "log" "Log";
-              p_copy true "rwset" "log" "Log") in
+      let p_reset () = p_commit_reset "Log" "log" in
+      let p_commit () = p_commit_reset "log" "Log" in
 
       let p_declare_target = function
         | VarTarget ({ tau; declared = false; name } as ti) ->
@@ -1466,15 +1506,14 @@ let compile (type pos_t var_t fn_name_t rule_name_t reg_t ext_fn_t)
   let buf_hpp = with_output_to_buffer p_hpp in
   (buf_hpp, buf_cpp)
 
-let cpp_rule_of_action all_regs (rl_name, (kind, rl_body)) =
-  let rl_footprint =
-    Array.of_list (Cuttlebone.Util.action_footprint all_regs rl_body) in
-  { rl_external = kind = `ExternalRule; rl_name; rl_body; rl_footprint }
+let cpp_rule_of_action reg_histories (rl_name, (kind, rl_body)) =
+  { rl_external = kind = `ExternalRule; rl_name; rl_body;
+    rl_reg_histories = reg_histories rl_name }
 
 let input_of_compile_unit (cu: 'f Cuttlebone.Compilation.compile_unit) =
   let rulemap r =
     snd (List.assoc r cu.c_rules) in
-  let annotated_rules, register_kinds =
+  let reg_histories, annotated_rules, register_kinds =
     Cuttlebone.Util.compute_register_histories
       Cuttlebone.Compilation._R cu.c_registers
       (List.map fst cu.c_rules) rulemap cu.c_scheduler in
@@ -1489,7 +1528,7 @@ let input_of_compile_unit (cu: 'f Cuttlebone.Compilation.compile_unit) =
     cpp_fn_names = (fun x -> x);
     cpp_rule_names = (fun ?prefix:_ rl -> rl);
     cpp_scheduler = cu.c_scheduler;
-    cpp_rules = List.map (cpp_rule_of_action cu.c_registers << swap_body) cu.c_rules;
+    cpp_rules = List.map (cpp_rule_of_action reg_histories << swap_body) cu.c_rules;
     cpp_registers = Array.of_list cu.c_registers;
     cpp_register_sigs = (fun r -> r);
     cpp_register_kinds = register_kinds;
@@ -1497,10 +1536,9 @@ let input_of_compile_unit (cu: 'f Cuttlebone.Compilation.compile_unit) =
     cpp_extfuns = cu.c_cpp_preamble; }
 
 let cpp_rule_of_koika_package_rule (kp: _ Extr.koika_package_t)
-      (annotated_rules: 'rn -> _) (rn: 'rn) =
+      (reg_histories: 'rn -> 'rg -> _) (annotated_rules: 'rn -> _) (rn: 'rn) =
   let kind rn = if kp.koika_rule_external rn then `ExternalRule else `InternalRule in
-  cpp_rule_of_action kp.koika_reg_finite.finite_elements
-    (rn, (kind rn, annotated_rules rn))
+  cpp_rule_of_action reg_histories (rn, (kind rn, annotated_rules rn))
 
 let input_of_sim_package
       (kp: ('pos_t, 'var_t, 'fn_name_t, 'rule_name_t, 'reg_t, 'ext_fn_t) Extr.koika_package_t)
@@ -1508,7 +1546,7 @@ let input_of_sim_package
     : ('pos_t, 'var_t, 'fn_name_t, 'rule_name_t, 'reg_t, 'ext_fn_t) cpp_input_t =
   let rule_names =
     Extr.scheduler_rules kp.koika_scheduler |> Cuttlebone.Util.dedup in
-  let annotated_rules, register_kinds =
+  let reg_histories, annotated_rules, register_kinds =
     Cuttlebone.Util.compute_register_histories
       kp.koika_reg_types kp.koika_reg_finite.finite_elements
       rule_names kp.koika_rules kp.koika_scheduler in
@@ -1523,7 +1561,7 @@ let input_of_sim_package
     cpp_rule_names = (fun ?prefix:_ rn ->
       Cuttlebone.Util.string_of_coq_string (kp.koika_rule_names.show0 rn));
     cpp_scheduler = kp.koika_scheduler;
-    cpp_rules = List.map (cpp_rule_of_koika_package_rule kp annotated_rules) rule_names;
+    cpp_rules = List.map (cpp_rule_of_koika_package_rule kp reg_histories annotated_rules) rule_names;
     cpp_registers = Array.of_list registers;
     cpp_register_sigs = Cuttlebone.Util.reg_sigs_of_koika_package kp;
     cpp_register_kinds = register_kinds;
